Capless/Inversion/Subtyping.lean
@@ -1,4 +1,6 @@
 import Capless.Subtyping
+import Capless.Store
+import Capless.Inversion.Basic
 namespace Capless
 
 theorem ESubtyp.sub_type_inv'
@@ -15,8 +17,72 @@ theorem ESubtyp.sub_type_inv
   ∃ T1, E1 = EType.type T1 ∧ CSubtyp Γ T1 T2 := by
   apply ESubtyp.sub_type_inv' rfl h
 
--- theorem SSubtyp.sub_forall_inv
---   (h : SSubtyp Γ S1 (SType.forall T E)) :
---   ∃
+def SSubtyp.dealias_right_forall.emotive
+  (Γ : Context n m k)
+  (E1 : EType n m k)
+  (E2 : EType n m k)
+  : Prop := True
+
+def SSubtyp.dealias_right_forall.cmotive
+  (Γ : Context n m k)
+  (C1 : CType n m k)
+  (C2 : CType n m k)
+  : Prop := True
+
+def SSubtyp.dealias_right_forall.smotive
+  (Γ : Context n m k)
+  (S1 : SType n m k)
+  (S2 : SType n m k)
+  : Prop :=
+  ∀ {T2 E2} (ht : Γ.IsTight) (hd : SType.Dealias Γ S2 (SType.forall T2 E2)),
+    ∃ T1 E1, SType.Dealias Γ S1 (SType.forall T1 E1)
+
+theorem SSubtyp.dealias_right_forall
+  (h : SSubtyp Γ S1 S2) (ht : Γ.IsTight)
+  (hd : SType.Dealias Γ S2 (SType.forall T2 E2)) :
+  ∃ T1 E1, SType.Dealias Γ S1 (SType.forall T1 E1) := by
+  apply SSubtyp.rec
+    (motive_1 := fun Γ E1 E2 h => SSubtyp.dealias_right_forall.emotive Γ E1 E2)
+    (motive_2 := fun Γ C1 C2 h => SSubtyp.dealias_right_forall.cmotive Γ C1 C2)
+    (motive_3 := fun Γ S1 S2 h => SSubtyp.dealias_right_forall.smotive Γ S1 S2)
+    (t := h) (hd := hd) (ht := ht)
+  case exist =>
+    unfold dealias_right_forall.cmotive dealias_right_forall.emotive
+    aesop
+  case type =>
+    unfold dealias_right_forall.cmotive dealias_right_forall.emotive
+    aesop
+  case capt =>
+    unfold dealias_right_forall.cmotive
+    aesop
+  case top =>
+    unfold dealias_right_forall.smotive
+    repeat intro
+    rename_i hd
+    cases hd
+  case refl =>
+    unfold dealias_right_forall.smotive
+    repeat intro
+    rename_i T2 E2 _ _
+    exists T2, E2
+  case trans =>
+    unfold dealias_right_forall.smotive
+    repeat intro
+    rename_i ih1 ih2 T3 E3 ht3 hd3
+    have ih2 := ih2 ht3 hd3
+    have ⟨T2, E2, hd2⟩ := ih2
+    have ih1 := ih1 ht3 hd2
+    exact ih1
+  case tvar =>
+    unfold dealias_right_forall.smotive
+    repeat intro
+    rename_i hb _ _ ht _
+    sorry
+  case tinstl => sorry
+  case tinstr => sorry
+  case xforall => sorry
+  case tforall => sorry
+  case cforall => sorry
+  case boxed => sorry
 
 end Capless
