Capless.lean
@@ -1,39 +1,86 @@
-import «Capless».Basic
+/-
+# Mechanisation of Capless
 
--- Syntax
+This is the entry of the mechanisation of System Capless.
+
+## Syntax
+-/
 import «Capless».CaptureSet
 import «Capless».Type
 import «Capless».Term
 import «Capless».Context
 
--- Static semantics
+/-
+## Static Semantics
+-/
 import «Capless».Subcapturing
 import «Capless».Subtyping
-import «Capless».Subtyping
+import «Capless».Typing
 
--- Operational semantics
+/-
+## Dynamic Semantics
+-/
 import «Capless».Store
 import «Capless».Reduction
 
--- Renaming
---- Term
+/-
+## The First Layer of Substitution Theorems: Renaming
+### Term Variable Renaming
+-/
 import «Capless».Renaming.Term.Subcapturing
 import «Capless».Renaming.Term.Subtyping
 import «Capless».Renaming.Term.Typing
---- Type
+/-
+### Type Variable Renaming
+-/
 import «Capless».Renaming.Type.Subcapturing
 import «Capless».Renaming.Type.Subtyping
 import «Capless».Renaming.Type.Typing
---- Capture
+/-
+### Capture Variable Renaming
+-/
 import «Capless».Renaming.Capture.Subcapturing
 import «Capless».Renaming.Capture.Subtyping
 import «Capless».Renaming.Capture.Typing
 
--- Substitution
---- Term
+/-
+## The Second Layer of Substitution Theorems: Substitution
+### Term Variable Substitution
+-/
 import «Capless».Subst.Term.Subcapturing
 import «Capless».Subst.Term.Subtyping
 import «Capless».Subst.Term.Typing
+/-
+### Type Variable Substitution
+-/
+import «Capless».Subst.Type.Subcapturing
+import «Capless».Subst.Type.Subtyping
+import «Capless».Subst.Type.Typing
+/-
+### Capture Variable Substitution
+-/
+import «Capless».Subst.Capture.Subcapturing
+import «Capless».Subst.Capture.Subtyping
+import «Capless».Subst.Capture.Typing
+
+/-
+## Inversion Theorems
+### Store Lookup
+It is mainly composed of the following results:
+- The type of the value stored in the store matches that in the corresponding typing context.
+-/
+import «Capless».Inversion.Lookup
+/-
+### Subtyping
+-/
+import «Capless».Inversion.Subtyping
+/-
+### Typing
+Main results:
+- Inversion of redex typing. For instance, an application `x y `is well-typed implies
+  that x is typed at a function and y can be typed at the argument type of the function.
+-/
+import «Capless».Inversion.Typing
 
 -- Soundness
 import «Capless».Soundness.Preservation
