Capless/Inversion/Basic.lean
@@ -1,0 +1,13 @@
+import Capless.Context
+
+namespace Capless
+
+inductive SType.Dealias : Context n m k -> SType n m k -> SType n m k -> Prop where
+| refl :
+  Dealias Γ S S
+| step :
+  Context.TBound Γ X (TBinding.inst S) ->
+  Dealias Γ S S' ->
+  Dealias Γ (SType.tvar X) S'
+
+end Capless
