Capless/Inversion/Context.lean
@@ -1,4 +1,5 @@
 import Capless.Context
+import Capless.Store
 namespace Capless
 
 theorem Context.var_bound_succ_inv'
@@ -16,5 +17,77 @@ theorem Context.var_bound_succ_inv
   (hb : Context.Bound (Γ.var P) x.succ T) :
   ∃ T0, Context.Bound Γ x T0 ∧ T = T0.weaken :=
   Context.var_bound_succ_inv' rfl rfl hb
+
+theorem Context.var_tbound_inv'
+  (he : Γ0 = Γ.var P)
+  (hb : Context.TBound Γ0 X b) :
+  ∃ b0, Context.TBound Γ X b0 ∧ b = b0.weaken := by
+  cases hb <;> try (solve | cases he)
+  case there_var b0 _ hb0 => cases he; exists b0
+
+theorem Context.var_tbound_inv
+  (hb : Context.TBound (Γ.var P) X b) :
+  ∃ b0, Context.TBound Γ X b0 ∧ b = b0.weaken :=
+  Context.var_tbound_inv' rfl hb
+
+theorem Context.var_tbound_inv_bound
+  (hb : Context.TBound (Γ.var P) X (TBinding.bound S)) :
+  ∃ S0, Context.TBound Γ X (TBinding.bound S0) ∧ S = SType.weaken S0 := by
+  have h := Context.var_tbound_inv hb
+  have ⟨b0, hb0, he0⟩ := h
+  cases b0
+  case bound S0 =>
+    simp [TBinding.weaken, TBinding.rename] at he0
+    simp [SType.weaken]
+    exists S0
+  case inst => simp [TBinding.weaken, TBinding.rename] at he0
+
+theorem Context.tinst_tbound_bound_inv'
+  (he1 : Γ0 = Γ.tvar (TBinding.inst P))
+  (he2 : b0 = TBinding.bound S)
+  (hb : Context.TBound Γ0 X b0) :
+  ∃ X0 S0, Context.TBound Γ X0 (TBinding.bound S0)
+    ∧ S = SType.tweaken S0
+    ∧ X = X0.succ := by
+  cases hb <;> try (solve | cases he1 | cases he2)
+  case here =>
+    cases he1
+    simp [TBinding.tweaken, TBinding.rename] at he2
+    cases he2
+  case there_tvar hb0 =>
+    cases he1
+    rename_i X0 b0
+    cases b0 <;> simp [TBinding.tweaken, TBinding.trename] at he2
+    rename_i S0
+    apply Exists.intro X0
+    apply Exists.intro S0
+    constructor <;> try constructor
+    { trivial }
+    { simp [SType.tweaken]; aesop }
+    { trivial }
+
+theorem Context.tinst_tbound_bound_inv
+  (hb : Context.TBound (Γ.tvar (TBinding.inst P)) X (TBinding.bound S)) :
+  ∃ X0 S0, Context.TBound Γ X0 (TBinding.bound S0)
+    ∧ S = SType.tweaken S0
+    ∧ X = X0.succ :=
+  Context.tinst_tbound_bound_inv' rfl rfl hb
+
+theorem Context.cvar_tbound_inv
+  (hb : Context.TBound (Γ.cvar p) X b) :
+  ∃ b0, Context.TBound Γ X b0 ∧ b = b0.cweaken := sorry
+
+theorem Context.tight_bound_tvar_absurd
+  (ht : Context.IsTight Γ)
+  (hb : Context.TBound Γ X (TBinding.bound S)) : False := by
+  induction ht
+  case empty => cases hb
+  case var ih =>
+    have ⟨S0, hb0, he0⟩ := Context.var_tbound_inv_bound hb
+    aesop
+  case tvar =>
+    have ⟨X0, S0, hb0, hs0, hx0⟩ := Context.tinst_tbound_bound_inv hb
+    aesop
+  case cvar => sorry
 
 end Capless
